src/program_proof/rsm/spaxos_propose.v
@@ -1,4 +1,26 @@
 From Perennial.program_proof.rsm Require Import spaxos_prelude.
+From Perennial.program_proof Require Import std_proof.
+
+Section fin_maps.
+Context `{FinMap K M}.
+
+Lemma map_intersection_subseteq {A : Type} (m1 m2 : M A) :
+  m1 ∩ m2 ⊆ m1.
+Proof using EqDecision0 H H0 H1 H2 H3 H4 H5 H6 K M.
+  rewrite !map_subseteq_spec. intros i x Hm.
+  rewrite lookup_intersection_Some in Hm.
+  by destruct Hm as [? _].
+Qed.
+
+Lemma lookup_insert_alter {A : Type} (f : A -> A) (m : M A) (i : K) (x : A) :
+  m !! i = Some x ->
+  <[i := f x]> m = alter f i m.
+Proof using EqDecision0 H H0 H1 H2 H3 H4 H5 H6 K M.
+  intros Hmi.
+  by rewrite -alter_insert insert_id.
+Qed.
+
+End fin_maps.
 
 (* TODO: move this out to spaxos_iris_inv.v once stable. *)
 Section inv.
@@ -50,6 +72,14 @@ Admitted.
 Definition know_sapxos_inv γ : iProp Σ :=
   inv spaxosN (spaxos_inv γ).
 
+Definition is_proposal_nz γ n v : iProp Σ :=
+  (if decide (n = O) then True else is_proposal γ n v)%I.
+
+#[global]
+Instance is_proposal_nz_persistent γ n v :
+  Persistent (is_proposal_nz γ n v).
+Proof. unfold is_proposal_nz. case_decide; apply _. Qed.
+
 End inv.
 
 #[export]
@@ -65,6 +95,8 @@ Context `{!heapGS Σ, !spaxos_ghostG Σ}.
 (*@ type Paxos struct {                                                     @*)
 (*@     // Mutex protecting all but @peers.                                 @*)
 (*@     mu      *sync.Mutex                                                 @*)
+(*@     // Node ID.                                                         @*)
+(*@     nid     uint64                                                      @*)
 (*@     // Term this paxos instance is currently in.                        @*)
 (*@     termc   uint64                                                      @*)
 (*@     // Term in which the currently accepted proposal is made.           @*)
@@ -80,6 +112,7 @@ Definition own_paxos (paxos : loc) (nid : Z) γ : iProp Σ :=
   ∃ (termc termp : u64) (decree : string) (learned : bool) (blt : ballot),
     (*@ Res: termc uint64                                                       @*)
     "Htermc" ∷ paxos ↦[Paxos :: "termc"] #termc ∗
+    "%Hnz"   ∷ ⌜int.nat termc ≠ O⌝ ∗
     (*@ Res: termp uint64                                                       @*)
     "Htermp" ∷ paxos ↦[Paxos :: "termp"] #termp ∗
     (*@ Res: decree string                                                      @*)
@@ -88,36 +121,41 @@ Definition own_paxos (paxos : loc) (nid : Z) γ : iProp Σ :=
     "Hlearned" ∷ paxos ↦[Paxos :: "learned"] #learned ∗
     (*@ Res: ballot ghost                                                       @*)
     "Hballot" ∷ own_ballot γ nid blt ∗
-    (*@ Res: termmap ghost                                                      @*)
-    "Hterm" ∷ own_term γ nid (int.nat termc) ∗
+    (*@ Res: termp uint64 / termmap ghost                                       @*)
+    "Hterm" ∷ own_term γ nid (int.nat termp) ∗
+    (*@ Res: termp uint64 / decree string / proposal ghost                      @*)
+    "#Hproposed" ∷ is_proposal_nz γ (int.nat termp) decree ∗
     (*@ Res: termc uint64 / ballot ghost                                        @*)
-    "%HballotLen" ∷ ⌜length blt = int.nat termc⌝ ∗
+    "%Hcurrent" ∷ ⌜length blt = int.nat termc⌝ ∗
     (*@ Res: termp uint64 / ballot ghost                                        @*)
-    "%HlastAcpt" ∷ True.
+    "%Hlatest" ∷ ⌜latest_term blt = (int.nat termp)⌝.
 
-Definition is_paxos_node (paxos : loc) (nid : Z) γ : iProp Σ :=
-  ∃ (mu : loc),
+(* TODO: figure the clean way of defining node ID. *)
+Definition is_paxos_node (paxos : loc) (nid : Z) (clst : gset Z) γ : iProp Σ :=
+  ∃ (mu : loc) (nidu64 : u64),
     (*@ Res: mu *sync.Mutex                                                     @*)
     "#Hmu"   ∷ readonly (paxos ↦[Paxos :: "mu"] #mu) ∗
-    "#Hlock" ∷ is_lock spaxosN #mu (own_paxos paxos nid γ).
+    "#Hlock" ∷ is_lock spaxosN #mu (own_paxos paxos nid γ) ∗
+    (*@ Res: nid uint64                                                         @*)
+    "#Hnid"  ∷ readonly (paxos ↦[Paxos :: "nid"] #nidu64) ∗
+    "%HnidZ" ∷ ⌜int.Z nidu64 = nid⌝ ∗
+    (*@ Res: cluster ghost                                                      @*)
+    "#Hcluster" ∷ is_cluster γ clst ∗
+    (*@ Res: ginv                                                               @*)
+    "#Hinv"  ∷ know_sapxos_inv γ.
 
 Definition is_paxos_comm (paxos : loc) (clst : gset Z) γ : iProp Σ :=
   ∃ (peers : Slice.t) (peersL : list loc),
     (*@ Res: peers []*Paxos                                                     @*)
     "#Hpeers"  ∷ readonly (paxos ↦[Paxos :: "peers"] (to_val peers)) ∗
     "#HpeersL" ∷ readonly (own_slice_small peers ptrT 1 peersL) ∗
-    (* For now we're using list index as node id, but might need another indirection later. *)
-    "#Hpaxos"  ∷ ([∗ list] i ↦ px ∈ peersL, is_paxos_node px (Z.of_nat i) γ) ∗
-    (* This looks ugly; think if there's better way to define this. *)
+    "#Hpaxos"  ∷ ([∗ list] i ↦ px ∈ peersL, is_paxos_node px (Z.of_nat i) clst γ) ∗
     "%Hclsteq" ∷ ⌜clst = list_to_set (Z.of_nat <$> (seq O (length peersL)))⌝.
 
 Definition is_paxos (paxos : loc) (nid : Z) γ : iProp Σ :=
   ∃ (clst : gset Z),
-    "#Hcluster" ∷ is_cluster γ clst ∗
-    "#Hnode"    ∷ is_paxos_node paxos nid γ ∗
-    "#Hcomm"    ∷ is_paxos_comm paxos clst γ ∗
-    "#Hinv"     ∷ know_sapxos_inv γ.
-
+    "#Hnode"    ∷ is_paxos_node paxos nid clst γ ∗
+    "#Hcomm"    ∷ is_paxos_comm paxos clst γ.
 End repr.
 
 #[export]
@@ -153,186 +191,61 @@ Proof.
   (*@ }                                                                       @*)
 Admitted.
 
-Definition P_Paxos__advance (px : loc) (termc : u64) nid γ: iProp Σ :=
-  "Htermc" ∷ px ↦[Paxos :: "termc"] #termc ∗
-  "Hterm"  ∷ own_term γ nid (int.nat termc).
+Definition node_prepared (term termp : u64) (decree : string) nid γ : iProp Σ :=
+  ∃ (l : ballot),
+    "#Hlb"     ∷ is_ballot_lb γ nid l ∗
+    "#Hdecree" ∷ is_proposal_nz γ (int.nat termp) decree ∗
+    "%Hlen"    ∷ ⌜(int.nat term ≤ length l)%nat⌝ ∗
+    "%Hlatest" ∷ ⌜latest_before (int.nat term) l = int.nat termp⌝.
 
-Definition Q_Paxos__advance (px : loc) (termc termold : u64) nid γ: iProp Σ :=
-  "Htermc"   ∷ px ↦[Paxos :: "termc"] #termc ∗
-  "Hterm"    ∷ own_term γ nid (int.nat termold) ∗
-  "%HtermLt" ∷ ⌜(int.nat termold < int.nat termc)%nat⌝ ∗
-  "%Hnode"   ∷ ⌜is_term_of_node nid (int.nat termc)⌝.
-
-Theorem wp_Paxos__proceedToNewTerm px termc nid γ :
-  {{{ P_Paxos__advance px termc nid γ }}}
-    Paxos__proceedToNewTerm #px
-  {{{ (term : u64), RET #term; Q_Paxos__advance px term termc nid γ }}}.
-Proof.
-  (*@ func (px *Paxos) proceedToNewTerm() uint64 {                            @*)
-  (*@     // TODO                                                             @*)
-  (*@     return 0                                                            @*)
-  (*@ }                                                                       @*)
-Admitted.
-
-Definition quorum_prepares
-  (term termp : u64) (decree : string) (clst : gset Z) (γ : spaxos_names) : iProp Σ :=
-  ∃ (bsqlb : gmap Z ballot),
-    "#Hlbs"      ∷ ([∗ map] x ↦ l ∈ bsqlb, is_ballot_lb γ x l) ∗
-    "#Hproposal" ∷ (if decide (int.nat termp = O) then True else is_proposal γ (int.nat termp) decree) ∗
-    "%Hquorum"   ∷ ⌜quorum clst (dom bsqlb)⌝ ∗
-    "%Hlen"      ∷ ⌜map_Forall (λ _ l, ((int.nat term) ≤ length l)%nat) bsqlb⌝ ∗
-    "%Hlargest"  ∷ ⌜latest_before_quorum (int.nat term) bsqlb = int.nat termp⌝.
-
-#[global]
-Instance quorum_prepares_persistent term termp decree clst γ :
-  Persistent (quorum_prepares term termp decree clst γ).
-Proof. unfold quorum_prepares. case_decide; apply _. Qed.
-
-Theorem wp_Paxos__prepareAll (px : loc) (term : u64) clst γ :
-  is_paxos_comm px clst γ -∗
+Theorem wp_Paxos__prepare (px : loc) (term : u64) nid clst γ :
+  is_paxos_node px nid clst γ -∗
   {{{ True }}}
-    Paxos__prepareAll #px #term
+    Paxos__prepare #px #term
   {{{ (termp : u64) (decree : string) (ok : bool), RET (#termp, #(LitString decree), #ok);
-      if ok then quorum_prepares term termp decree clst γ else True
+      if ok then node_prepared term termp decree nid γ else True
   }}}.
 Proof.
-  (*@ func (px *Paxos) prepareAll(term uint64) (uint64, string, bool) {       @*)
-  (*@     var termLargest uint64                                              @*)
-  (*@     var decreeLargest string                                            @*)
-  (*@     var nPrepared uint64                                                @*)
-  (*@     for _, peer := range(px.peers) {                                    @*)
-  (*@         // Send each node a prepare message.                            @*)
-  (*@         termPeer, decreePeer, ok := peer.prepare(term)                  @*)
-  (*@         if ok {                                                         @*)
-  (*@             nPrepared++                                                 @*)
-  (*@             if termPeer > termLargest {                                 @*)
-  (*@                 // Update the largest-term proposal we've seen.         @*)
-  (*@                 termLargest = termPeer                                  @*)
-  (*@                 decreeLargest = decreePeer                              @*)
-  (*@             }                                                           @*)
-  (*@         }                                                               @*)
-  (*@     }                                                                   @*)
-  (*@                                                                         @*)
-  (*@     // Did not reach a majority.                                        @*)
-  (*@     if !px.major(nPrepared) {                                           @*)
-  (*@         return 0, "", false                                             @*)
-  (*@     }                                                                   @*)
-  (*@                                                                         @*)
-  (*@     return termLargest, decreeLargest, true                             @*)
-  (*@ }                                                                       @*)
-Admitted.
-
-Definition quorum_accepts (term : u64) (clst : gset Z) (γ : spaxos_names) : iProp Σ :=
-  ∃ (bsqlb : gmap Z ballot),
-    "#Hlbs"     ∷ ([∗ map] x ↦ l ∈ bsqlb, is_ballot_lb γ x l) ∗
-    "%Hquorum"  ∷ ⌜quorum clst (dom bsqlb)⌝ ∗
-    "%Haccin"   ∷ ⌜map_Forall (λ _ l, accepted_in l (int.nat term)) bsqlb⌝.
-
-#[global]
-Instance quorum_accepts_persistent term clst γ :
-  Persistent (quorum_accepts γ term clst).
-Proof. apply _. Qed.
-
-Theorem wp_Paxos__acceptAll (px : loc) (term : u64) (decree : string) clst γ :
-  is_paxos_comm px clst γ -∗
-  is_proposal γ (int.nat term) decree -∗
-  {{{ True }}}
-    Paxos__acceptAll #px #term #(LitString decree)
-  {{{ (ok : bool), RET #ok; if ok then quorum_accepts term clst γ else True }}}.
-Proof.
-  (*@ func (px *Paxos) acceptAll(term uint64, decree string) bool {           @*)
-  (*@     var nAccepted uint64 = 0                                            @*)
-  (*@     for _, peer := range(px.peers) {                                    @*)
-  (*@         ok := peer.accept(term, decree)                                 @*)
-  (*@         if ok {                                                         @*)
-  (*@             nAccepted++                                                 @*)
-  (*@         }                                                               @*)
-  (*@     }                                                                   @*)
-  (*@                                                                         @*)
-  (*@     return px.major(nAccepted)                                          @*)
-  (*@ }                                                                       @*)
-Admitted.
-
-Theorem wp_Paxos__learnAll (px : loc) (term : u64) (decree : string) clst γ :
-  is_paxos_comm px clst γ -∗
-  is_chosen_consensus γ decree -∗
-  {{{ True }}}
-    Paxos__learnAll #px #term #(LitString decree)
-  {{{ RET #(); True }}}.
-Proof.
-  (*@ func (px *Paxos) learnAll(term uint64, decree string) {                 @*)
-  (*@     for _, peer := range(px.peers) {                                    @*)
-  (*@         peer.learn(term, decree)                                        @*)
-  (*@     }                                                                   @*)
-  (*@ }                                                                       @*)
-Admitted.
-
-Lemma ite_apply (A B : Type) (b : bool) (f : A -> B) x y :
-  (if b then f x else f y) = f (if b then x else y).
-Proof. destruct b; done. Qed.
-
-End temp.
-(* TODO: move them out to their own files once stable. *)
-
-Section fin_maps.
-Context `{FinMap K M}.
-
-Lemma map_intersection_subseteq {A : Type} (m1 m2 : M A) :
-  m1 ∩ m2 ⊆ m1.
-Proof using EqDecision0 H H0 H1 H2 H3 H4 H5 H6 K M.
-  rewrite !map_subseteq_spec. intros i x Hm.
-  rewrite lookup_intersection_Some in Hm.
-  by destruct Hm as [? _].
-Qed.
-
-Lemma lookup_insert_alter {A : Type} (f : A -> A) (m : M A) (i : K) (x : A) :
-  m !! i = Some x ->
-  <[i := f x]> m = alter f i m.
-Proof using EqDecision0 H H0 H1 H2 H3 H4 H5 H6 K M.
-  intros Hmi.
-  by rewrite -alter_insert insert_id.
-Qed.
-
-End fin_maps.
-
-Section prog.
-Context `{!heapGS Σ, !spaxos_ghostG Σ}.
-
-Theorem wp_Paxos__Propose (px : loc) (v : string) nid γ :
-  is_paxos px nid γ -∗
-  {{{ True }}}
-    Paxos__Propose #px #(LitString v)
-  {{{ (ok : bool), RET #ok; if ok then is_proposed_decree γ v else True }}}.
-Proof.
-  iIntros "#Hpaxos !>" (Φ) "_ HΦ".
-  iNamed "Hpaxos".
-  iNamed "Hnode".
+  iIntros "#Hnode" (Φ) "!> _ HΦ".
   wp_call.
 
-  (*@ func (px *Paxos) Propose(v string) bool {                               @*)
+  (*@ func (px *Paxos) prepare(term uint64) (uint64, string, bool) {          @*)
   (*@     px.mu.Lock()                                                        @*)
   (*@                                                                         @*)
+  iNamed "Hnode".
   wp_loadField.
   wp_apply (acquire_spec with "[$Hlock]").
   iIntros "[Hlocked HpaxosOwn]".
   wp_pures.
-  
-  (*@     // Proceed to a new term exclusively owned by this paxos node.      @*)
-  (*@     // NB: Raft does not exclusively own a term until the first phase goes thru. @*)
-  (*@     term := px.proceedToNewTerm()                                       @*)
+
+  (*@     if term < px.termc {                                                @*)
+  (*@         px.mu.Unlock()                                                  @*)
+  (*@         return 0, "", false                                             @*)
+  (*@     }                                                                   @*)
   (*@                                                                         @*)
   iNamed "HpaxosOwn".
-  wp_apply (wp_Paxos__proceedToNewTerm with "[$Htermc $Hterm]").
-  iIntros (term) "Hpost".
-  iNamed "Hpost".
-  wp_pures.
+  wp_loadField.
+  wp_if_destruct.
+  { wp_loadField.
+    wp_apply (release_spec with "[-HΦ $Hlock $Hlocked]"); first by eauto 15 with iFrame.
+    wp_pures.
+    by iApply "HΦ".
+  }
 
+  (*@     px.termc = term                                                     @*)
+  (*@                                                                         @*)
+  wp_storeField.
+
+  (*@     // Ghost action:                                                    @*)
+  (*@     // Extending the ballot of this node with [false] to @term to extract a @*)
+  (*@     // promise that this node won't accept any proposal before @term.   @*)
+  (*@                                                                         @*)
   set blt' := extend false (int.nat term) blt.
   iAssert (|={⊤}=> own_ballot γ nid blt')%I with "[Hballot]" as "> Hballot".
   { iInv "Hinv" as ">HinvO" "HinvC".
     iNamed "HinvO".
     iDestruct (ballot_lookup with "Hballot Hbs") as %Hblt.
-    iMod (ballot_update (extend false (int.nat term) blt) with "Hballot Hbs") as "[Hballot Hbs]".
+    iMod (ballot_update blt' with "Hballot Hbs") as "[Hballot Hbs]".
     { apply extend_prefix. }
     rewrite lookup_insert_alter; last done.
     pose proof (vb_inv_prepare nid (int.nat term) Hvbs) as Hvbs'.
@@ -340,114 +253,364 @@ Proof.
     pose proof (vc_inv_prepare nid (int.nat term) Hvc) as Hvc'.
     by iMod ("HinvC" with "[Hc Hbs Hps Hts]") as "_"; first by eauto 15 with iFrame.
   }
+  iDestruct (ballot_witness with "Hballot") as "#Hbltlb".
 
-  (*@     // Phase 1.                                                         @*)
-  (*@     // Goals of this phase is to get a quorum of nodes:                 @*)
-  (*@     // (1) promise not to accept any proposal with term below @term, and @*)
-  (*@     // (2) find out the largest proposal (below @term) accepted by the quorum. @*)
-  (*@     termLargest, decreeLargest, prepared := px.prepareAll(term)         @*)
+  (*@     termp  := px.termp                                                  @*)
+  (*@     decree := px.decree                                                 @*)
   (*@                                                                         @*)
-  wp_apply (wp_Paxos__prepareAll with "Hcomm").
-  iIntros (termLargest decreeLargest prepared) "Hprepares".
+  do 2 wp_loadField.
   wp_pures.
-  
-  (*@     if !prepared {                                                      @*)
+
+  (*@     px.mu.Unlock()                                                      @*)
+  (*@                                                                         @*)
+  wp_loadField.
+  wp_apply (release_spec with "[-HΦ $Hlock $Hlocked]").
+  { do 5 iExists _. iFrame "∗ #".
+    iPureIntro.
+    split; first lia.
+    split.
+    { rewrite extend_length. lia. }
+    by rewrite latest_term_extend_false.
+  }
+  wp_pures.
+
+  (*@     // Informally, a positive response (@t, @d, @true) of @prepare(n) means: @*)
+  (*@     // (1) This node will not accept any proposal with term below @n, and @*)
+  (*@     // (2) The largest-term proposal this node has accepted before term @n is @*)
+  (*@     // decree (@t, @d).                                                 @*)
+  (*@     return termp, decree, true                                          @*)
+  (*@ }                                                                       @*)
+  iApply "HΦ".
+  iExists _.
+  iFrame "# %".
+  iPureIntro.
+  split.
+  { rewrite extend_length. lia. }
+  replace (int.nat term) with (length blt'); last first.
+  { rewrite extend_length. lia. }
+  rewrite -Hlatest.
+  replace (latest_before _ _) with (latest_term blt') by done.
+  apply latest_term_extend_false.
+Qed.
+
+Theorem wp_Paxos__advance (px : loc) nid clst γ :
+  is_paxos_node px nid clst γ -∗
+  {{{ True }}}
+    Paxos__advance #px
+  {{{ (term : u64) (termp : u64) (decree : string), RET (#term, #termp, #(LitString decree));
+      node_prepared term termp decree nid γ ∗ ⌜is_term_of_node nid (int.nat term) ∧ int.nat term ≠ O⌝
+  }}}.
+Proof.
+  iIntros "#Hnode" (Φ) "!> _ HΦ".
+  wp_call.
+
+  (*@ func (px *Paxos) advance() (uint64, uint64, string) {                   @*)
+  (*@     px.mu.Lock()                                                        @*)
+  (*@                                                                         @*)
+  iNamed "Hnode".
+  wp_loadField.
+  wp_apply (acquire_spec with "[$Hlock]").
+  iIntros "[Hlocked HpaxosOwn]".
+  wp_pures.
+
+  (*@     term := std.SumAssumeNoOverflow(px.termc, MAX_NODES) / MAX_NODES * MAX_NODES + px.nid @*)
+  (*@                                                                         @*)
+  iNamed "HpaxosOwn".
+  wp_loadField.
+  wp_apply wp_SumAssumeNoOverflow.
+  iIntros (Hoverflow).
+  wp_pures.
+  wp_loadField.
+  wp_pures.
+  set term := (word.add _ _).
+  assert (Hofnode : is_term_of_node nid (int.nat term)).
+  { admit. }
+  assert (Hlt : (int.nat termc < int.nat term)%nat).
+  { admit. }
+
+  (*@     px.termc = term                                                     @*)
+  (*@                                                                         @*)
+  wp_storeField.
+
+  (*@     // Ghost action:                                                    @*)
+  (*@     // Extending the ballot of this node with [false] to @term to extract a @*)
+  (*@     // promise that this node won't accept any proposal before @term.   @*)
+  (*@                                                                         @*)
+  set blt' := extend false (int.nat term) blt.
+  iAssert (|={⊤}=> own_ballot γ nid blt')%I with "[Hballot]" as "> Hballot".
+  { iInv "Hinv" as ">HinvO" "HinvC".
+    iNamed "HinvO".
+    iDestruct (ballot_lookup with "Hballot Hbs") as %Hblt.
+    iMod (ballot_update blt' with "Hballot Hbs") as "[Hballot Hbs]".
+    { apply extend_prefix. }
+    rewrite lookup_insert_alter; last done.
+    pose proof (vb_inv_prepare nid (int.nat term) Hvbs) as Hvbs'.
+    pose proof (vp_inv_prepare nid (int.nat term) Hvps) as Hvps'.
+    pose proof (vc_inv_prepare nid (int.nat term) Hvc) as Hvc'.
+    by iMod ("HinvC" with "[Hc Hbs Hps Hts]") as "_"; first by eauto 15 with iFrame.
+  }
+  iDestruct (ballot_witness with "Hballot") as "#Hbltlb".
+
+  (*@     termp  := px.termp                                                  @*)
+  (*@     decree := px.decree                                                 @*)
+  (*@                                                                         @*)
+  do 2 wp_loadField.
+  wp_pures.
+
+  (*@     px.mu.Unlock()                                                      @*)
+  (*@                                                                         @*)
+  wp_loadField.
+  wp_apply (release_spec with "[-HΦ $Hlock $Hlocked]").
+  { do 5 iExists _. iFrame "∗ #".
+    iPureIntro.
+    split; first lia.
+    split.
+    { rewrite extend_length. lia. }
+    by rewrite latest_term_extend_false.
+  }
+  wp_pures.
+
+  (*@     return term, termp, decree                                          @*)
+  (*@ }                                                                       @*)
+  iApply "HΦ".
+  iModIntro.
+  iSplit; last first.
+  { iPureIntro. split; [done | lia]. }
+  iExists _.
+  iFrame "# %".
+  iPureIntro.
+  split.
+  { rewrite extend_length. lia. }
+  replace (int.nat term) with (length blt'); last first.
+  { rewrite extend_length. lia. }
+  rewrite -Hlatest.
+  replace (latest_before _ _) with (latest_term blt') by done.
+  apply latest_term_extend_false.
+Admitted.
+
+Definition node_accepted (term : u64) (decree : string) nid γ : iProp Σ :=
+  ∃ (l : ballot),
+    "#Hlb"    ∷ is_ballot_lb γ nid l ∗
+    "%Haccin" ∷ ⌜accepted_in l (int.nat term)⌝.
+
+Theorem wp_Paxos__accept (px : loc) (term : u64) (decree : string) nid clst γ :
+  is_paxos_node px nid clst γ -∗
+  is_proposal γ (int.nat term) decree -∗
+  {{{ True }}}
+    Paxos__accept #px #term #(LitString decree)
+  {{{ (ok : bool), RET #ok; if ok then node_accepted term decree nid γ else True }}}.
+Proof.
+  iIntros "#Hnode #Hproposal" (Φ) "!> _ HΦ".
+  wp_call.
+
+  (*@ func (px *Paxos) accept(term uint64, decree string) bool {              @*)
+  (*@     px.mu.Lock()                                                        @*)
+  (*@                                                                         @*)
+  iNamed "Hnode".
+  wp_loadField.
+  wp_apply (acquire_spec with "[$Hlock]").
+  iIntros "[Hlocked HpaxosOwn]".
+  wp_pures.
+
+  (*@     if term < px.termc {                                                @*)
   (*@         px.mu.Unlock()                                                  @*)
   (*@         return false                                                    @*)
   (*@     }                                                                   @*)
   (*@                                                                         @*)
+  iNamed "HpaxosOwn".
+  wp_loadField.
   wp_if_destruct.
   { wp_loadField.
-    (* XXX: should not need below after relating term map to termp rather than termc. *)
-    iApply fupd_wp.
-    iInv "Hinv" as ">HinvO" "HinvC".
-    iNamed "HinvO".
-    iDestruct (term_lookup with "Hterm Hts") as %Htermc.
-    assert (Hprev : gt_prev_term ts nid (int.nat term)).
-    { exists (int.nat termc). split; [done | word]. }
-    iMod (term_update (int.nat term) with "Hterm Hts") as "[Hterm Hts]".
-    pose proof (vt_inv_advance Hprev Hvts) as Hvts'.
-    iMod ("HinvC" with "[Hc Hbs Hps Hts]") as "_"; first by eauto 15 with iFrame.
-    iModIntro.
-    wp_apply (release_spec with "[-HΦ $Hlock $Hlocked]").
-    { do 5 iExists _. iFrame. iPureIntro. rewrite extend_length. lia. }
+    wp_apply (release_spec with "[-HΦ $Hlock $Hlocked]"); first by eauto 15 with iFrame.
     wp_pures.
     by iApply "HΦ".
   }
-  iDestruct "Hprepares" as "#Hprepares".
-  
-  (*@     // If @termLargest is not set (meaning no node in the quorum has accepted @*)
-  (*@     // any proposal yet), we can propose our value @v.                  @*)
-  (*@     var decree string                                                   @*)
-  (*@     var helping bool                                                    @*)
+
+  (*@     px.termc = std.SumAssumeNoOverflow(term, 1)                         @*)
+  (*@     px.termp = term                                                     @*)
+  (*@     px.decree = decree                                                  @*)
   (*@                                                                         @*)
-  wp_apply (wp_ref_of_zero); first done.
-  iIntros (decreeRef) "HdecreeRef".
-  wp_pures.
-  wp_apply (wp_ref_of_zero); first done.
-  iIntros (helpingRef) "HhelpingRef".
+  wp_apply wp_SumAssumeNoOverflow.
+  iIntros (Hoverflow).
+  do 3 wp_storeField.
+
+  (*@     // Ghost action:                                                    @*)
+  (*@     // Extending the ballot of this node with [false] to @term and append one @*)
+  (*@     // [true] at index @term.                                           @*)
+  (*@                                                                         @*)
+  set accept := λ l, (extend false (int.nat term) l) ++ [true].
+  set blt' := accept blt.
+  set R := (own_ballot γ nid blt' ∗ own_term γ nid (int.nat term))%I.
+  iAssert (|={⊤}=> R)%I with "[Hballot Hterm]" as "> [Hballot Hterm]".
+  { iInv "Hinv" as ">HinvO" "HinvC".
+    iNamed "HinvO".
+    iDestruct (ballot_lookup with "Hballot Hbs") as %Hblt.
+    iDestruct (proposal_lookup with "Hproposal Hps") as %Hpsl.
+    iDestruct (term_lookup with "Hterm Hts") as %Htm.
+    assert (Hprev : gt_prev_term ts nid (int.nat term)).
+    { exists (int.nat termp). split; first done.
+      assert (int.nat termp < int.nat termc)%nat.
+      { rewrite -Hcurrent -Hlatest. apply latest_before_lt. lia. }
+      lia.
+    }
+    iMod (ballot_update blt' with "Hballot Hbs") as "[Hballot Hbs]".
+    { apply prefix_app_r, extend_prefix. }
+    rewrite lookup_insert_alter; last done.
+    iMod (term_update (int.nat term) with "Hterm Hts") as "[Hterm Hts]".
+    unshelve epose proof (vb_inv_accept nid (int.nat term) _ _ Hvbs) as Hvbs'.
+    { done. }
+    { exists blt. split; first done. lia. }
+    pose proof (vp_inv_accept nid (int.nat term) Hvps) as Hvps'.
+    pose proof (vc_inv_accept nid (int.nat term) Hvc) as Hvc'.
+    pose proof (vt_inv_advance Hprev Hvts) as Hvts'.
+    iMod ("HinvC" with "[Hc Hbs Hps Hts]") as "_"; first by eauto 15 with iFrame.
+    by iFrame.
+  }
+  clear R.
+  iDestruct (ballot_witness with "Hballot") as "#Hbltlb".
+
+  (*@     px.mu.Unlock()                                                      @*)
+  (*@                                                                         @*)
+  wp_loadField.
+  iClear "Hproposed".
+  iAssert (is_proposal_nz γ (int.nat term) decree)%I as "#Hproposed".
+  { unfold is_proposal_nz. case_decide; done. }
+  wp_apply (release_spec with "[-HΦ $Hlock $Hlocked]").
+  { do 5 iExists _. iFrame "∗ #".
+    iPureIntro.
+    replace (int.nat (word.add _ _)) with (S (int.nat term)) by word.
+    split; first done.
+    split.
+    { rewrite last_length extend_length. lia. }
+    rewrite latest_term_snoc_true extend_length.
+    lia.
+  }
   wp_pures.
 
-  (*@     if termLargest == 0 {                                               @*)
-  (*@         // We're the ``initiating'' thread.                             @*)
-  (*@         decree = v                                                      @*)
-  (*@         helping = false                                                 @*)
-  (*@     } else {                                                            @*)
-  (*@         // We're the ``helping'' thread.                                @*)
-  (*@         decree = decreeLargest                                          @*)
-  (*@         helping = true                                                  @*)
+  (*@     return true                                                         @*)
+  (*@ }                                                                       @*)
+  iApply "HΦ".
+  iExists _.
+  iFrame "#".
+  iPureIntro.
+  unfold accepted_in.
+  split; last lia.
+  rewrite lookup_app_r; last first.
+  { rewrite extend_length. lia. }
+  rewrite extend_length.
+  by replace (_ - _)%nat with O by lia.
+Qed.
+
+Definition quorum_prepared
+  (term : u64) (terml : u64) (decreel : string) (clst : gset Z) (γ : spaxos_names) : iProp Σ :=
+  ∃ (bsqlb : gmap Z ballot),
+    "#Hlbs"      ∷ ([∗ map] x ↦ l ∈ bsqlb, is_ballot_lb γ x l) ∗
+    "#Hproposal" ∷ is_proposal_nz γ (int.nat terml) decreel ∗
+    "%Hquorum"   ∷ ⌜quorum clst (dom bsqlb)⌝ ∗
+    "%Hlen"      ∷ ⌜map_Forall (λ _ l, ((int.nat term) ≤ length l)%nat) bsqlb⌝ ∗
+    "%Hlargest"  ∷ ⌜latest_before_quorum (int.nat term) bsqlb = int.nat terml⌝.
+
+#[global]
+Instance quorum_prepared_persistent term terml decree clst γ :
+  Persistent (quorum_prepared term terml decree clst γ).
+Proof. apply _. Qed.
+
+Theorem wp_Paxos__accept__proposer
+  (px : loc) (term : u64) (decree : string) (terml : u64) decreel nid clst γ :
+  is_term_of_node nid (int.nat term) ->
+  (if decide (int.nat terml = O) then True else decree = decreel) ->
+  quorum_prepared term terml decreel clst γ -∗
+  is_paxos_node px nid clst γ -∗
+  {{{ True }}}
+    Paxos__accept #px #term #(LitString decree)
+  {{{ (ok : bool), RET #ok;
+      if ok then node_accepted term decree nid γ ∗ is_proposal γ (int.nat term) decree else True
+  }}}.
+Proof.
+  iIntros "%Hofnode %Hdecree #Hprepares #Hnode" (Φ) "!> _ HΦ".
+  wp_call.
+
+  (*@ func (px *Paxos) accept(term uint64, decree string) bool {              @*)
+  (*@     px.mu.Lock()                                                        @*)
+  (*@                                                                         @*)
+  iNamed "Hnode".
+  wp_loadField.
+  wp_apply (acquire_spec with "[$Hlock]").
+  iIntros "[Hlocked HpaxosOwn]".
+  wp_pures.
+
+  (*@     if term < px.termc {                                                @*)
+  (*@         px.mu.Unlock()                                                  @*)
+  (*@         return false                                                    @*)
   (*@     }                                                                   @*)
   (*@                                                                         @*)
-  wp_apply (wp_If_join_evar with "[HdecreeRef HhelpingRef]").
-  { iIntros (b Eqb).
-    case_bool_decide.
-    - wp_if_true.
-      do 2 wp_store.
-      iModIntro.
-      iSplit; first done.
-      replace (LitString v) with
-        (if b then (LitString v) else (LitString decreeLargest)) by by rewrite Eqb.
-      replace #false with #(if b then false else true) by by rewrite Eqb.
-      iNamedAccu.
-    - wp_if_false.
-      do 2 wp_store.
-      iModIntro.
-      iSplit; first done.
-      rewrite Eqb.
-      by iFrame.
+  iNamed "HpaxosOwn".
+  wp_loadField.
+  wp_if_destruct.
+  { wp_loadField.
+    wp_apply (release_spec with "[-HΦ $Hlock $Hlocked]"); first by eauto 15 with iFrame.
+    wp_pures.
+    by iApply "HΦ".
   }
-  iIntros "Hdh".
-  iNamed "Hdh".
-  wp_pures.
-  (* Push [LitString] and [LitBool] out for [Hdecree] and [Hhelping], respectively. *)
-  do 2 rewrite ite_apply.
+  iClear "Hproposed".
 
-  (*@     // Now that we have decided what to propose (i.e., @decree), we can perform @*)
-  (*@     // a ghost update on [proposals]. To do so in an invariant-preserving way, @*)
-  (*@     // we need to know two things:                                      @*)
-  (*@     // 1. @term has not been proposed, and                              @*)
-  (*@     // 2. the proposal we're making, (@term, @decree), is a valid one.  @*)
-  (*@     // See [vp_inv_propose] for detail.                                 @*)
+  (*@     px.termc = std.SumAssumeNoOverflow(term, 1)                         @*)
+  (*@     px.termp = term                                                     @*)
+  (*@     px.decree = decree                                                  @*)
   (*@                                                                         @*)
-  assert (Hnz : (int.nat term) ≠ O) by lia.
-  rename decree into decree_prev.
-  set decree := (if (bool_decide _) then v else _).
+  wp_apply wp_SumAssumeNoOverflow.
+  iIntros (Hoverflow).
+  do 3 wp_storeField.
+
+  (*@     // Ghost action for proposer:                                       @*)
+  (*@     // (1) updating termmap of this node to @term,                      @*)
+  (*@     // (2) inserting proposal (@term, @decree) in proposals.            @*)
+  (*@     //                                                                  @*)
+  (*@     // Note 1:                                                          @*)
+  (*@     // To update the proposals in an invariant-preserving way, we need to know @*)
+  (*@     // two things:                                                      @*)
+  (*@     // (1) @term has not been used, and                                 @*)
+  (*@     // (2) the proposal we're making, (@term, @decree), is a valid one. @*)
+  (*@     // See [vp_inv_propose] for detail.                                 @*)
+  (*@     //                                                                  @*)
+  (*@     // Note 2: Ideally, we want to update the ghost state one at a time if @*)
+  (*@     // possible; for instance, we update the termmap and proposals here, and @*)
+  (*@     // then the ballot below.                                           @*)
+  (*@     // Following this discipline should significatly simplify invairance proofs. @*)
+  (*@     // However, sometimes we'll have to update more than one ghost states in one @*)
+  (*@     // step; for instance, we update the termmap and proposals together @*)
+  (*@     // here. The reason is that we need to deduce @term is free using the @*)
+  (*@     // free-term invariant, insert the proposal at @term, update the termmap @*)
+  (*@     // entry to @term to re-establish the free-term invariant.          @*)
+  (*@     //                                                                  @*)
+  (*@     // Note 3: An alternative design would be separately proposing and then @*)
+  (*@     // accepting. The downside of this design is that we would need an  @*)
+  (*@     // additional physical state to distinguish between "not proposed" state @*)
+  (*@     // from "proposed but not accepted" state. By merging proposing with @*)
+  (*@     // accepting, we know a term has not been used by a node if that term @*)
+  (*@     // belongs to the node *and* that the node has not accepted the term. Hence @*)
+  (*@     // this design saves one physical state.                            @*)
+  (*@                                                                         @*)
+  assert (Htermcp : (int.nat termp < int.nat termc)%nat).
+  { rewrite -Hcurrent -Hlatest. apply latest_before_lt. lia. }
+  assert (Htermorder : (int.nat termp < int.nat term)%nat) by lia.
   set R := (own_term γ nid (int.nat term) ∗ is_proposal γ (int.nat term) decree)%I.
-  iAssert (|={⊤}=> R)%I with "[Hterm]" as "> [Hterm #Hp]".
+  iAssert (|={⊤}=> R)%I with "[Hterm]" as "> [Hterm #Hproposal]".
   { iInv "Hinv" as ">HinvO" "HinvC".
     iNamed "HinvO".
     iDestruct (term_lookup with "Hterm Hts") as %Htermc.
     assert (Hprev : gt_prev_term ts nid (int.nat term)).
-    { exists (int.nat termc). split; [done | word]. }
-    pose proof (vt_impl_freshness Htermc HtermLt Hnode Hvts) as Hfresh.
+    { exists (int.nat termp). split; [done | word]. }
+    pose proof (vt_impl_freshness Htermc Htermorder Hofnode Hvts) as Hfresh.
     iAssert (⌜valid_proposal bs ps (int.nat term) decree⌝)%I as %Hvalid.
     { iNamed "Hprepares".
-      iDestruct (ballots_prefix with "Hlbs Hbs") as "%Hprefix".
-      iAssert (⌜if decide (int.nat termLargest = O)
+      iDestruct (ballots_prefix with "Hlbs Hbs") as %Hprefix.
+      unfold is_proposal_nz.
+      iAssert (⌜if decide (int.nat terml = O)
                then True
-               else ps !! (int.nat termLargest) = Some decreeLargest⌝)%I as "%Hatterm".
-      { case_decide; [done | by iApply proposal_lookup]. }
-      iDestruct (cluster_eq with "Hcluster Hclst") as "->".
+               else ps !! (int.nat terml) = Some decree⌝)%I as %Hatterm.
+      { case_decide; first done. rewrite Hdecree. by iApply proposal_lookup. }
+      iDestruct (cluster_eq with "Hcluster Hclst") as %->.
       iPureIntro.
       set bsq := bs ∩ bsqlb.
       exists bsq.
@@ -483,65 +646,307 @@ Proof.
       }
       case_decide as Hcase.
       - left. by rewrite Hcase in Hlargest.
-      - right. rewrite Hlargest.
-        subst decree.
-        case_bool_decide as Hcontra; last done.
-        clear -Hcase Hcontra.
-        (* Set Printing Coercions. *)
-        inversion Hcontra as [Hzero].
-        rewrite Hzero in Hcase.
-        unfold int.nat in Hcase.
-        replace (int.Z _) with 0 in Hcase; word.
+      - right. by rewrite Hlargest.
     }
     iMod (proposals_insert _ _ decree with "Hps") as "[Hps #Hp]"; first apply Hfresh.
     iMod (term_update (int.nat term) with "Hterm Hts") as "[Hterm Hts]".
-    pose proof (vp_inv_propose Hfresh Hnz Hvalid Hvps) as Hvps'.
+    assert (Htermnz : int.nat term ≠ O) by lia.
+    pose proof (vp_inv_propose Hfresh Htermnz Hvalid Hvps) as Hvps'.
     pose proof (vb_inv_propose (int.nat term) decree Hvbs) as Hvbs'.
     pose proof (vc_inv_propose (int.nat term) decree Hvc) as Hvc'.
-    pose proof (vt_inv_propose_advance decree Hprev Hnode Hvts) as Hvts'.
+    pose proof (vt_inv_propose_advance decree Hprev Hofnode Hvts) as Hvts'.
     iMod ("HinvC" with "[Hc Hbs Hps Hts]") as "_"; first by eauto 10 with iFrame.
     by iFrame.
   }
   clear R.
+
+  (*@     // Ghost action:                                                    @*)
+  (*@     // Extending the ballot of this node with [false] to @term and append one @*)
+  (*@     // [true] at index @term.                                           @*)
+  (*@                                                                         @*)
+  set accept := λ l, (extend false (int.nat term) l) ++ [true].
+  set blt' := accept blt.
+  iAssert (|={⊤}=> own_ballot γ nid blt')%I with "[Hballot]" as "> Hballot".
+  { iInv "Hinv" as ">HinvO" "HinvC".
+    iNamed "HinvO".
+    iDestruct (ballot_lookup with "Hballot Hbs") as %Hblt.
+    iDestruct (proposal_lookup with "Hproposal Hps") as %Hpsl.
+    iMod (ballot_update blt' with "Hballot Hbs") as "[Hballot Hbs]".
+    { apply prefix_app_r, extend_prefix. }
+    rewrite lookup_insert_alter; last done.
+    unshelve epose proof (vb_inv_accept nid (int.nat term) _ _ Hvbs) as Hvbs'.
+    { done. }
+    { exists blt. split; first done. lia. }
+    pose proof (vp_inv_accept nid (int.nat term) Hvps) as Hvps'.
+    pose proof (vc_inv_accept nid (int.nat term) Hvc) as Hvc'.
+    iMod ("HinvC" with "[Hc Hbs Hps Hts]") as "_"; first by eauto 15 with iFrame.
+    by iFrame.
+  }
+  iDestruct (ballot_witness with "Hballot") as "#Hbltlb".
+
+  (*@     px.mu.Unlock()                                                      @*)
+  (*@                                                                         @*)
+  wp_loadField.
+  iAssert (is_proposal_nz γ (int.nat term) decree)%I as "#Hproposed".
+  { unfold is_proposal_nz. destruct (decide (int.nat term = _)); done. }
+  wp_apply (release_spec with "[-HΦ $Hlock $Hlocked]").
+  { do 5 iExists _. iFrame "∗ #".
+    iPureIntro.
+    replace (int.nat (word.add _ _)) with (S (int.nat term)) by word.
+    split; first done.
+    split.
+    { rewrite last_length extend_length. lia. }
+    rewrite latest_term_snoc_true extend_length.
+    lia.
+  }
+  wp_pures.
+
+  (*@     return true                                                         @*)
+  (*@ }                                                                       @*)
+  iApply "HΦ". iModIntro.
+  iSplit; last done.
+  iExists _.
+  iFrame "#".
+  iPureIntro.
+  unfold accepted_in.
+  split; last lia.
+  rewrite lookup_app_r; last first.
+  { rewrite extend_length. lia. }
+  rewrite extend_length.
+  by replace (_ - _)%nat with O by lia.
+Qed.
+
+Theorem wp_Paxos__prepareAll (px : loc) (term terma : u64) (decreea : string) clst nid γ :
+  is_paxos_comm px clst γ -∗
+  node_prepared term terma decreea nid γ -∗
+  {{{ True }}}
+    Paxos__prepareAll #px #term #terma #(LitString decreea)
+  {{{ (termp : u64) (decree : string) (ok : bool), RET (#termp, #(LitString decree), #ok);
+      if ok then quorum_prepared term termp decree clst γ else True
+  }}}.
+Proof.
+  (*@ func (px *Paxos) prepareAll(term uint64) (uint64, string, bool) {       @*)
+  (*@     var termLargest uint64                                              @*)
+  (*@     var decreeLargest string                                            @*)
+  (*@     var nPrepared uint64                                                @*)
+  (*@     for _, peer := range(px.peers) {                                    @*)
+  (*@         // Send each node a prepare message.                            @*)
+  (*@         termPeer, decreePeer, ok := peer.prepare(term)                  @*)
+  (*@         if ok {                                                         @*)
+  (*@             nPrepared++                                                 @*)
+  (*@             if termPeer > termLargest {                                 @*)
+  (*@                 // Update the largest-term proposal we've seen.         @*)
+  (*@                 termLargest = termPeer                                  @*)
+  (*@                 decreeLargest = decreePeer                              @*)
+  (*@             }                                                           @*)
+  (*@         }                                                               @*)
+  (*@     }                                                                   @*)
+  (*@                                                                         @*)
+  (*@     // Did not reach a majority.                                        @*)
+  (*@     if !px.major(nPrepared) {                                           @*)
+  (*@         return 0, "", false                                             @*)
+  (*@     }                                                                   @*)
+  (*@                                                                         @*)
+  (*@     return termLargest, decreeLargest, true                             @*)
+  (*@ }                                                                       @*)
+Admitted.
+
+Definition quorum_accepted (term : u64) (clst : gset Z) (γ : spaxos_names) : iProp Σ :=
+  ∃ (bsqlb : gmap Z ballot),
+    "#Hlbs"    ∷ ([∗ map] x ↦ l ∈ bsqlb, is_ballot_lb γ x l) ∗
+    "%Hquorum" ∷ ⌜quorum clst (dom bsqlb)⌝ ∗
+    "%Haccin"  ∷ ⌜map_Forall (λ _ l, accepted_in l (int.nat term)) bsqlb⌝.
+
+#[global]
+Instance quorum_accepted_persistent term clst γ :
+  Persistent (quorum_accepted γ term clst).
+Proof. apply _. Qed.
+
+Theorem wp_Paxos__acceptAll (px : loc) (term : u64) (decree : string) clst nid γ :
+  is_paxos_comm px clst γ -∗
+  node_accepted term decree nid γ -∗
+  is_proposal γ (int.nat term) decree -∗
+  {{{ True }}}
+    Paxos__acceptAll #px #term #(LitString decree)
+  {{{ (ok : bool), RET #ok; if ok then quorum_accepted term clst γ else True }}}.
+Proof.
+  (*@ func (px *Paxos) acceptAll(term uint64, decree string) bool {           @*)
+  (*@     var nAccepted uint64 = 0                                            @*)
+  (*@     for _, peer := range(px.peers) {                                    @*)
+  (*@         ok := peer.accept(term, decree)                                 @*)
+  (*@         if ok {                                                         @*)
+  (*@             nAccepted++                                                 @*)
+  (*@         }                                                               @*)
+  (*@     }                                                                   @*)
+  (*@                                                                         @*)
+  (*@     return px.major(nAccepted)                                          @*)
+  (*@ }                                                                       @*)
+Admitted.
+
+Theorem wp_Paxos__learnAll (px : loc) (term : u64) (decree : string) clst γ :
+  is_paxos_comm px clst γ -∗
+  is_chosen_consensus γ decree -∗
+  {{{ True }}}
+    Paxos__learnAll #px #term #(LitString decree)
+  {{{ RET #(); True }}}.
+Proof.
+  (*@ func (px *Paxos) learnAll(term uint64, decree string) {                 @*)
+  (*@     for _, peer := range(px.peers) {                                    @*)
+  (*@         peer.learn(term, decree)                                        @*)
+  (*@     }                                                                   @*)
+  (*@ }                                                                       @*)
+Admitted.
+
+Lemma ite_apply (A B : Type) (b : bool) (f : A -> B) x y :
+  (if b then f x else f y) = f (if b then x else y).
+Proof. destruct b; done. Qed.
+
+End temp.
+
+Section prog.
+Context `{!heapGS Σ, !spaxos_ghostG Σ}.
+
+Theorem wp_Paxos__Propose (px : loc) (v : string) nid γ :
+  is_paxos px nid γ -∗
+  {{{ True }}}
+    Paxos__Propose #px #(LitString v)
+  {{{ (ok : bool), RET #ok; if ok then is_proposed_decree γ v else True }}}.
+Proof.
+  iIntros "#Hpaxos !>" (Φ) "_ HΦ".
+  wp_call.
+
+  (*@ func (px *Paxos) Propose(v string) bool {                               @*)
+  (*@     // Proceed to a new term exclusively owned by this paxos node.      @*)
+  (*@     // NB: Raft does not exclusively own a term until the first phase goes thru. @*)
+  (*@     term, terma, decreea := px.advance()                                @*)
+  (*@                                                                         @*)
+  iNamed "Hpaxos".
+  wp_apply (wp_Paxos__advance with "Hnode").
+  iIntros (term terma decreea) "[#Hprep [%Hofnode %Htermnz]]".
+  wp_pures.
+
+  (*@     // Phase 1.                                                         @*)
+  (*@     // Goals of this phase is to get a quorum of nodes:                 @*)
+  (*@     // (1) promise not to accept any proposal with term below @term, and @*)
+  (*@     // (2) find out the largest proposal (below @term) accepted by the quorum. @*)
+  (*@     terml, decreel, prepared := px.prepareAll(term, terma, decreea)     @*)
+  (*@                                                                         @*)
+  wp_apply (wp_Paxos__prepareAll with "Hcomm Hprep").
+  iIntros (terml decreel prepared) "Hprepq".
+  wp_pures.
+  
+  (*@     if !prepared {                                                      @*)
+  (*@         return false                                                    @*)
+  (*@     }                                                                   @*)
+  (*@                                                                         @*)
+  wp_if_destruct; first by iApply "HΦ".
+  iDestruct "Hprepq" as "#Hprepq".
+
+  (*@     var decree string                                                   @*)
+  (*@     var helping bool                                                    @*)
+  (*@                                                                         @*)
+  wp_apply (wp_ref_of_zero); first done.
+  iIntros (decreeRef) "HdecreeRef".
+  wp_pures.
+  wp_apply (wp_ref_of_zero); first done.
+  iIntros (helpingRef) "HhelpingRef".
+  wp_pures.
+
+  (*@     // If @terml is not set (meaning no node in the quorum has accepted any @*)
+  (*@     // proposal yet), we can propose our value @v.                      @*)
+  (*@     if terml == 0 {                                                     @*)
+  (*@         // We're the ``initiating'' thread.                             @*)
+  (*@         decree = v                                                      @*)
+  (*@         helping = false                                                 @*)
+  (*@     } else {                                                            @*)
+  (*@         // We're the ``helping'' thread.                                @*)
+  (*@         decree = decreel                                                @*)
+  (*@         helping = true                                                  @*)
+  (*@     }                                                                   @*)
+  (*@                                                                         @*)
+  wp_apply (wp_If_join_evar with "[HdecreeRef HhelpingRef]").
+  { iIntros (b Eqb).
+    case_bool_decide.
+    - wp_if_true.
+      do 2 wp_store.
+      iModIntro.
+      iSplit; first done.
+      replace (LitString v) with
+        (if b then (LitString v) else (LitString decreel)) by by rewrite Eqb.
+      replace #false with #(if b then false else true) by by rewrite Eqb.
+      iNamedAccu.
+    - wp_if_false.
+      do 2 wp_store.
+      iModIntro.
+      iSplit; first done.
+      rewrite Eqb.
+      by iFrame.
+  }
+  iIntros "Hdh".
+  iNamed "Hdh".
+  wp_pures.
+  (* Push [LitString] and [LitBool] out for [Hdecree] and [Hhelping], respectively. *)
+  do 2 rewrite ite_apply.
+
+  (*@     // We have decided what to propose (i.e., @decree).                 @*)
+  (*@     proposed := px.accept(term, decree)                                 @*)
+  (*@                                                                         @*)
+  wp_load.
+  wp_apply (wp_Paxos__accept__proposer with "Hprepq Hnode"); first done.
+  { case_decide as Hneq; first done.
+    case_bool_decide as Heq; last done.
+    inversion Heq as [Eterml].
+    rewrite Eterml in Hneq.
+    by replace (int.nat (U64 0)) with O in Hneq by word.
+  }
+  iIntros (proposed) "Hproposed".
+  wp_pures.
+
+  (*@     if !proposed {                                                      @*)
+  (*@         return false                                                    @*)
+  (*@     }                                                                   @*)
+  (*@                                                                         @*)
+  wp_if_destruct; first by iApply "HΦ".
+  iDestruct "Hproposed" as "[#Hacpt #Hpsl]".
 
   (*@     // Phase 2.                                                         @*)
   (*@     // Goal of this phase is to get a quorum of nodes accepting our proposal. @*)
   (*@     accepted := px.acceptAll(term, decree)                              @*)
   (*@                                                                         @*)
   wp_load.
-  wp_apply (wp_Paxos__acceptAll with "Hcomm Hp").
-  iIntros (accepted) "Haccepts".
+  wp_apply (wp_Paxos__acceptAll with "Hcomm Hacpt Hpsl").
+  iIntros (accepted) "Hacptq".
   wp_pures.
-  
+
   (*@     if !accepted {                                                      @*)
-  (*@         px.mu.Unlock()                                                  @*)
   (*@         return !helping                                                 @*)
   (*@     }                                                                   @*)
   (*@                                                                         @*)
   wp_if_destruct.
-  { wp_loadField.
-    wp_apply (release_spec with "[-HΦ HhelpingRef $Hlock $Hlocked]").
-    { do 5 iExists _. iFrame. iPureIntro. rewrite extend_length. lia. }
-    wp_pures.
-    wp_load.
+  { wp_load.
     unfold is_proposed_decree.
     case_bool_decide; wp_pures; iApply "HΦ"; [by eauto | done].
   }
-  iDestruct "Haccepts" as "#Haccepts".
-  
+  iDestruct "Hacptq" as "#Hacptq".
+
+  (*@     // Ghost action: Committing the consensus.                          @*)
+  (*@     //                                                                  @*)
+  (*@     // Note 1:                                                          @*)
   (*@     // If @accepted is true, we know @decree is chosen either the first time, @*)
   (*@     // or has already been chosen earlier. If it's the first time, we simply @*)
   (*@     // perform a ghost update on consensus; if it's been chosen earlier, we @*)
   (*@     // apply the top-level consistency theorem to deduce the decree chosen here @*)
   (*@     // (i.e., @decree) is equal to the one chosen eariler.              @*)
   (*@                                                                         @*)
+  set decree := (if (bool_decide _) then v else _).
   iAssert (|={⊤}=> is_chosen_consensus γ decree)%I as "> #Hconsensus".
-  { iInv "Hinv" as ">HinvO" "HinvC".
+  { iNamed "Hnode".
+    iInv "Hinv" as ">HinvO" "HinvC".
     iNamed "HinvO".
     iAssert (⌜chosen bs ps decree⌝)%I as %Hchosen.
-    { iNamed "Haccepts".
+    { iNamed "Hacptq".
       iDestruct (ballots_prefix with "Hlbs Hbs") as %Hprefix.
-      iDestruct (proposal_lookup with "Hp Hps") as %Hatterm.
+      iDestruct (proposal_lookup with "Hpsl Hps") as %Hatterm.
       iDestruct (cluster_eq with "Hcluster Hclst") as %->.
       iPureIntro.
       exists (int.nat term).
@@ -588,26 +993,14 @@ Proof.
   wp_load.
   wp_apply (wp_Paxos__learnAll with "Hcomm Hconsensus").
   wp_pures.
-  
-  (*@     px.mu.Unlock()                                                      @*)
-  (*@                                                                         @*)
-  wp_loadField.
-  wp_apply (release_spec with "[-HΦ HhelpingRef $Hlock $Hlocked]").
-  { do 5 iExists _. iFrame. iPureIntro. rewrite extend_length. lia. }
-  wp_pures.
 
   (*@     // If @helping is true, return false since we're merely helping an early @*)
   (*@     // proposal go through, rather than proposing our own value @v.     @*)
   (*@     return !helping                                                     @*)
-  (*@                                                                         @*)
+  (*@ }                                                                       @*)
   wp_load.
   unfold is_proposed_decree.
   case_bool_decide; wp_pures; iApply "HΦ"; [by eauto | done].
-  
-  (*@     // Wait until consensus is reached.                                 @*)
-  (*@     // NB: Deferred consensus don't need this.                          @*)
-  (*@     // for !px.isLearned() { }                                          @*)
-  (*@ }                                                                       @*)
 Qed.
 
 End prog.
